types/coq/SosADL/Interpretation.v
@@ -54,6 +54,200 @@ Fixpoint interp_in_Z (e: SosADL.SosADL.t_Expression) {struct e} :=
     | _ => Failed e e
   end.
 
+Lemma interpInZ_unary o x (H: exists f, interp_in_Z (SosADL.SosADL.UnaryExpression (Some o) (Some x)) = Interpreted f):
+  o = "+" \/ o = "-".
+Proof.
+  destruct H as [ f H ].
+  simpl in H. destruct o; try discriminate.
+  destruct a.
+  destruct b; try discriminate;
+    destruct b0; try discriminate;
+      destruct b1; try discriminate;
+        destruct b2; try discriminate;
+          destruct b3; try discriminate;
+            destruct b4; try discriminate;
+              destruct b5; try discriminate;
+                destruct b6; try discriminate;
+                  destruct o; try discriminate;
+                    auto.
+Qed.
+
+Lemma interpInZ_unary_pos x (H: exists f, interp_in_Z (SosADL.SosADL.UnaryExpression (Some "+") (Some x)) = Interpreted f):
+  exists fx, interp_in_Z x = Interpreted fx.
+Proof.
+  destruct H as [ f H ].
+  simpl in H.
+  destruct (interp_in_Z x).
+  - exists z. auto.
+  - discriminate.
+Qed.
+
+Lemma interpInZ_unary_neg x (H: exists f, interp_in_Z (SosADL.SosADL.UnaryExpression (Some "-") (Some x)) = Interpreted f):
+  exists fx, interp_in_Z x = Interpreted fx.
+Proof.
+  destruct H as [ f H ].
+  simpl in H.
+  destruct (interp_in_Z x).
+  - exists z. auto.
+  - discriminate.
+Qed.
+
+Lemma interpInZ_binary x o y (H: exists f, interp_in_Z (SosADL.SosADL.BinaryExpression (Some x) (Some o) (Some y)) = Interpreted f):
+  o = "+" \/ o = "-" \/ o = "*" \/ o = "/" \/ o = "mod".
+Proof.
+  destruct H as [ f H ].
+  simpl in H. destruct o; try discriminate.
+  repeat (destruct a;
+          destruct b; try discriminate;
+          destruct b0; try discriminate;
+          destruct b1; try discriminate;
+          destruct b2; try discriminate;
+          destruct b3; try discriminate;
+          destruct b4; try discriminate;
+          destruct b5; try discriminate;
+          destruct b6; try discriminate;
+          destruct o; try discriminate;
+          auto).
+Qed.
+
+Lemma interpInZ_binary_add_l x y (H: exists f, interp_in_Z (SosADL.SosADL.BinaryExpression (Some x) (Some "+") (Some y)) = Interpreted f):
+  exists fx, interp_in_Z x = Interpreted fx.
+Proof.
+  destruct H as [ f H ].
+  simpl in H.
+  destruct (interp_in_Z x).
+  - exists z. auto.
+  - discriminate.
+Qed.
+
+Lemma interpInZ_binary_add_r x y (H: exists f, interp_in_Z (SosADL.SosADL.BinaryExpression (Some x) (Some "+") (Some y)) = Interpreted f):
+  exists fx, interp_in_Z y = Interpreted fx.
+Proof.
+  destruct H as [ f H ].
+  simpl in H.
+  destruct (interp_in_Z x).
+  - destruct (interp_in_Z y).
+    + exists z0. auto.
+    + discriminate.
+  - discriminate.
+Qed.
+
+Lemma interpInZ_binary_sub_l x y (H: exists f, interp_in_Z (SosADL.SosADL.BinaryExpression (Some x) (Some "-") (Some y)) = Interpreted f):
+  exists fx, interp_in_Z x = Interpreted fx.
+Proof.
+  destruct H as [ f H ].
+  simpl in H.
+  destruct (interp_in_Z x).
+  - exists z. auto.
+  - discriminate.
+Qed.
+
+Lemma interpInZ_binary_sub_r x y (H: exists f, interp_in_Z (SosADL.SosADL.BinaryExpression (Some x) (Some "-") (Some y)) = Interpreted f):
+  exists fx, interp_in_Z y = Interpreted fx.
+Proof.
+  destruct H as [ f H ].
+  simpl in H.
+  destruct (interp_in_Z x).
+  - destruct (interp_in_Z y).
+    + exists z0. auto.
+    + discriminate.
+  - discriminate.
+Qed.
+
+Lemma interpInZ_binary_mul_l x y (H: exists f, interp_in_Z (SosADL.SosADL.BinaryExpression (Some x) (Some "*") (Some y)) = Interpreted f):
+  exists fx, interp_in_Z x = Interpreted fx.
+Proof.
+  destruct H as [ f H ].
+  simpl in H.
+  destruct (interp_in_Z x).
+  - exists z. auto.
+  - discriminate.
+Qed.
+
+Lemma interpInZ_binary_mul_r x y (H: exists f, interp_in_Z (SosADL.SosADL.BinaryExpression (Some x) (Some "*") (Some y)) = Interpreted f):
+  exists fx, interp_in_Z y = Interpreted fx.
+Proof.
+  destruct H as [ f H ].
+  simpl in H.
+  destruct (interp_in_Z x).
+  - destruct (interp_in_Z y).
+    + exists z0. auto.
+    + discriminate.
+  - discriminate.
+Qed.
+
+Lemma interpInZ_binary_div_l x y (H: exists f, interp_in_Z (SosADL.SosADL.BinaryExpression (Some x) (Some "/") (Some y)) = Interpreted f):
+  exists fx, interp_in_Z x = Interpreted fx.
+Proof.
+  destruct H as [ f H ].
+  simpl in H.
+  destruct (interp_in_Z x).
+  - exists z. auto.
+  - discriminate.
+Qed.
+
+Lemma interpInZ_binary_div_r x y (H: exists f, interp_in_Z (SosADL.SosADL.BinaryExpression (Some x) (Some "/") (Some y)) = Interpreted f):
+  exists fx, interp_in_Z y = Interpreted fx.
+Proof.
+  destruct H as [ f H ].
+  simpl in H.
+  destruct (interp_in_Z x).
+  - destruct (interp_in_Z y).
+    + exists z0. auto.
+    + discriminate.
+  - discriminate.
+Qed.
+
+Lemma interpInZ_binary_mod_l x y (H: exists f, interp_in_Z (SosADL.SosADL.BinaryExpression (Some x) (Some "mod") (Some y)) = Interpreted f):
+  exists fx, interp_in_Z x = Interpreted fx.
+Proof.
+  destruct H as [ f H ].
+  simpl in H.
+  destruct (interp_in_Z x).
+  - exists z. auto.
+  - discriminate.
+Qed.
+
+Lemma interpInZ_binary_mod_r x y (H: exists f, interp_in_Z (SosADL.SosADL.BinaryExpression (Some x) (Some "mod") (Some y)) = Interpreted f):
+  exists fx, interp_in_Z y = Interpreted fx.
+Proof.
+  destruct H as [ f H ].
+  simpl in H.
+  destruct (interp_in_Z x).
+  - destruct (interp_in_Z y).
+    + exists z0. auto.
+    + discriminate.
+  - discriminate.
+Qed.
+
+Fixpoint interp_in_Z_ind (P: forall e, (exists f, interp_in_Z e = Interpreted f) -> Prop)
+           (Plit: forall x (H: exists f, interp_in_Z (SosADL.SosADL.IntegerValue (Some x)) = Interpreted f), P (SosADL.SosADL.IntegerValue (Some x)) H)
+           (Ppos: forall x (H: exists f, interp_in_Z (SosADL.SosADL.UnaryExpression (Some "+") (Some x)) = Interpreted f) (I: P x (interpInZ_unary_pos x H)), P (SosADL.SosADL.UnaryExpression (Some "+") (Some x)) H)
+           (Pneg: forall x (H: exists f, interp_in_Z (SosADL.SosADL.UnaryExpression (Some "-") (Some x)) = Interpreted f) (I: P x (interpInZ_unary_neg x H)), P (SosADL.SosADL.UnaryExpression (Some "-") (Some x)) H)
+           (Padd: forall x y (H: exists f, interp_in_Z (SosADL.SosADL.BinaryExpression (Some x) (Some "+") (Some y)) = Interpreted f) (I: P x (interpInZ_binary_add_l x y H)) (J: P y (interpInZ_binary_add_r x y H)), P (SosADL.SosADL.BinaryExpression (Some x) (Some "+") (Some y)) H)
+           (Psub: forall x y (H: exists f, interp_in_Z (SosADL.SosADL.BinaryExpression (Some x) (Some "-") (Some y)) = Interpreted f) (I: P x (interpInZ_binary_sub_l x y H)) (J: P y (interpInZ_binary_sub_r x y H)), P (SosADL.SosADL.BinaryExpression (Some x) (Some "-") (Some y)) H)
+           (Pmul: forall x y (H: exists f, interp_in_Z (SosADL.SosADL.BinaryExpression (Some x) (Some "*") (Some y)) = Interpreted f) (I: P x (interpInZ_binary_mul_l x y H)) (J: P y (interpInZ_binary_mul_r x y H)), P (SosADL.SosADL.BinaryExpression (Some x) (Some "*") (Some y)) H)
+           (Pdiv: forall x y (H: exists f, interp_in_Z (SosADL.SosADL.BinaryExpression (Some x) (Some "/") (Some y)) = Interpreted f) (I: P x (interpInZ_binary_div_l x y H)) (J: P y (interpInZ_binary_div_r x y H)), P (SosADL.SosADL.BinaryExpression (Some x) (Some "/") (Some y)) H)
+           (Pmod: forall x y (H: exists f, interp_in_Z (SosADL.SosADL.BinaryExpression (Some x) (Some "mod") (Some y)) = Interpreted f) (I: P x (interpInZ_binary_mod_l x y H)) (J: P y (interpInZ_binary_mod_r x y H)), P (SosADL.SosADL.BinaryExpression (Some x) (Some "mod") (Some y)) H)
+           e (H: exists f, interp_in_Z e = Interpreted f) {struct e}: P e H.
+  destruct e; try (destruct H; discriminate).
+  - destruct o; try (destruct H; discriminate).
+    destruct o0; try (destruct H; discriminate).
+    destruct o1; try (destruct H; discriminate).
+    destruct (interpInZ_binary _ _ _ H) as [ I | [ I | [ I | [ I | I ] ] ] ]; subst.
+    + apply Padd; apply interp_in_Z_ind; auto.
+    + apply Psub; apply interp_in_Z_ind; auto.
+    + apply Pmul; apply interp_in_Z_ind; auto.
+    + apply Pdiv; apply interp_in_Z_ind; auto.
+    + apply Pmod; apply interp_in_Z_ind; auto.
+  - destruct o; try (destruct H; discriminate). apply Plit.
+  - destruct o; try (destruct H; discriminate).
+    destruct o0; try (destruct H; discriminate).
+    destruct (interpInZ_unary _ _ H) as [ I | I ]; subst.
+    + apply Ppos; apply interp_in_Z_ind; auto.
+    + apply Pneg; apply interp_in_Z_ind; auto.
+Qed.
+
 (** * Comparison of expressions *)
 
 (** Currently, the sole way to prove comparison consists in
